coq/theories/utils/Llist.v
@@ -1,3 +1,10 @@
-CoInductive Llist (A : Type) : Type :=
-| Lnil : Llist A
-| Lcons : A -> Llist A -> Llist A.
+CoInductive llist {A : Type} : Type :=
+| lnil : llist
+| lcons : A -> llist -> llist.
+Arguments llist : clear implicits.
+
+Definition ltail {A : Type} (l : llist A) : llist A :=
+  match l with
+  | lnil => lnil
+  | lcons _ tl => tl
+  end.
