coq/theories/utils/Words64Naive.v
@@ -6,10 +6,6 @@ Require Import coqutil.Word.Bitwidth.
 
 Local Open Scope Z_scope.
 
-Definition word64 := word 64.
+Notation word64 := (word 64).
 
 #[global] Instance word64_instance: word.word 64 := Naive.word 64.
-
-#[global] Instance Words64Naive: Bitwidth 64 := {|
-  width_cases := or_intror eq_refl;
-|}.
