coq/TODOs.md
@@ -1,13 +1,5 @@
 TODO:
-- word4 – use coqutil
-- termination of c_cmd
+- llist – own co-inductive llist
 
 Nice to have:
 - Alias that isn't substituted everywhere? `name := nat` (not Notation)
-
-Done?:
-- char – used Coq.Strings.Ascii.ascii
-- word64 – used coqutil
-
-
-- llist – own co-inductive llist
